theories/sim/body.v
@@ -24,7 +24,7 @@ Proof.
     pclearbot. right. eapply CIH; eauto.
   - econstructor 2; eauto.
     intros.
-    destruct (CONT _ _ _ σs' σt' VRET STACK) as [idx' SIM'].
+    destruct (CONT _ _ _ σs' σt' VRET WSAT1 STACK) as [idx' SIM'].
     exists idx'. pclearbot.
     right. eapply CIH; eauto.
 Qed.
@@ -51,9 +51,10 @@ Proof.
     split; last split; [done|by rewrite cmra_assoc|].
     pclearbot. right. by eapply CIH.
   - econstructor 2; eauto.
-    { instantiate (1:= (rf ⋅ rc)). by rewrite -cmra_assoc (cmra_assoc r_f). }
+    { instantiate (1:= rf ⋅ rc). by rewrite -cmra_assoc (cmra_assoc r_f). }
     intros.
-    specialize (CONT _ _ _ σs' σt' VRET STACK) as [idx' SIM'].
+    specialize (CONT _ _ _ σs' σt' VRET) as [idx' SIM']; [|done|].
+    { move : WSAT1. by rewrite 3!cmra_assoc. }
     exists idx'. pclearbot. right. eapply CIH; eauto. by rewrite cmra_assoc.
 Qed.
 
@@ -155,8 +156,8 @@ Proof.
         { pclearbot. left. eapply paco7_mon_bot; eauto. }
       + eapply (sim_local_body_step_over_call _ _ _ _ _ _ _ _ _ _ _ _ _
             Ks1 Kt1 fid vl_tgt _ _ _ _ CALLTGT); eauto; [by etrans|].
-        intros r4 vs4 vt4 σs4 σt4 VREL4 STACK4.
-        destruct (CONT _ _ _ σs4 σt4 VREL4 STACK4) as [idx4 CONT4].
+        intros r4 vs4 vt4 σs4 σt4 VREL4 WSAT4 STACK4.
+        destruct (CONT _ _ _ σs4 σt4 VREL4 WSAT4 STACK4) as [idx4 CONT4].
         exists idx4. pclearbot. left.  eapply paco7_mon_bot; eauto.
     - (* et makes a step *)
       constructor 1. intros.
@@ -172,8 +173,8 @@ Proof.
     eapply (sim_local_body_step_over_call _ _ _ _ _ _ _ _ _ _ _ _ _
             (Ks1 ++ Ks) (Kt1 ++ Kt) fid vl_tgt); [by rewrite CALLTGT fill_app|..];
             eauto; [rewrite fill_app; by apply fill_tstep_rtc|].
-    intros r' vs' vt' σs' σt' VREL' STACK'.
-    destruct (CONT _ _ _ σs' σt' VREL' STACK') as [idx' CONT2]. clear CONT.
+    intros r' vs' vt' σs' σt' VREL' WSAT' STACK'.
+    destruct (CONT _ _ _ σs' σt' VREL' WSAT' STACK') as [idx' CONT2]. clear CONT.
     exists idx'. rewrite 2!fill_app.
     pclearbot. right. by apply CIH. }
 Qed.
