theories/sim/program.v
@@ -12,13 +12,16 @@ Lemma sim_prog_sim_classical
                              ~ terminal e' /\
                              ~ reducible prog_src e' σ'}
       (FUNS: sim_local_funs wsat vrel prog_src prog_tgt end_call_sat)
-      (MAINT: ∃ ebt HCt, prog_tgt !! "main" = Some (@FunV [] ebt HCt))
+      (MAINT: ∃ ebs HCs, prog_src !! "main" = Some (@FunV [] ebs HCs))
   : behave_prog prog_tgt <1= behave_prog prog_src.
 Proof.
-  destruct MAINT as (ebt & HCt & Eqt).
-  destruct (FUNS _ _ Eqt) as ([xls ebs HCs] & Eqs & Eql & SIMf).
+  destruct MAINT as (ebs & HCs & Eqs).
+  destruct (FUNS _ _ Eqs) as ([xlt ebt HCt] & Eqt & Eql & SIMf).
+  simpl in Eql. symmetry in Eql.
   apply nil_length_inv in Eql. simplify_eq/=.
-  specialize (SIMf ε ebs ebt [] [] init_state init_state) as [idx SIM]; [simpl; done..|].
+  specialize (SIMf ε ebs ebt [] [] init_state init_state) as [idx SIM];
+    [simpl; done..|].
+
   unfold behave_prog.
   eapply (adequacy_classical _ _ idx); [apply NSD| |by apply wf_init_state..].
   eapply sim_local_conf_sim; eauto.
@@ -40,7 +43,8 @@ Proof.
     have HL: (init_res ⋅ r').(rcm) !! 0%nat ≡ Some (to_callStateR csPub).
     { apply cmap_lookup_op_l_equiv_pub; [apply VALID|].
       by rewrite /= lookup_singleton. }
-    split. { destruct ((init_res ⋅ r').(rcm) !! 0%nat). by eexists. by inversion HL. }
+    split.
+    { destruct ((init_res ⋅ r').(rcm) !! 0%nat). by eexists. by inversion HL. }
     intros r_f VALIDf T HL2. exfalso.
     move : HL2. rewrite lookup_op HL. apply callStateR_exclusive_2.
   - instantiate (1:=ε). rewrite right_id left_id. apply wsat_init_state.
